src/Examples/Logging/HoareProof.v
@@ -1,0 +1,80 @@
+Require Import POCS.
+Require Import Spec.HoareTactics.
+
+Require Import Examples.Logging.Impl.
+Require Import Examples.Logging.LogLayout.
+Require Import Examples.Logging.LogicalLog.
+
+Local Notation proc_rspec := (Hoare.proc_rspec D.ODLayer.(sem)).
+Local Arguments Hoare.proc_rspec {Op State} sem {T R}.
+
+Definition logical_abstraction (d: D.State) ps ls :=
+  PhyDecode d ps /\
+  LogDecode ps ls /\
+  ls.(ls_committed) = false.
+
+Local Hint Resolve log_read_ok.
+Local Hint Resolve recovery_ok.
+Local Hint Resolve log_apply_spec_idempotent_crash_step_notxn.
+Local Hint Resolve log_apply_spec_idempotent_crash_step.
+
+Definition general_rspec T (p_cspec: Specification T unit D.State) :=
+  @proc_cspec_to_rspec _ _
+    D.ODLayer.(sem)
+                (PhysicalState*LogicalState) _ _ p_cspec
+                (fun '(ps, ls) => log_apply_spec ps ls ls.(ls_disk) ls.(ls_committed)).
+
+
+Definition mk_rspec ls0 T (p_cspec: Specification T unit D.State) :=
+  @proc_cspec_to_rspec _ _
+    D.ODLayer.(sem)
+                _ _ _ p_cspec
+                (fun (a: { '(ps, ls) | ls.(ls_disk) = ls0.(ls_disk) }) =>
+                   let 'exist _ (ps, ls) _ := a in
+                   log_apply_spec ps ls ls.(ls_disk) false).
+
+Definition log_read_rec_ok ps ls a :
+  proc_rspec
+    (log_read a)
+    (recovery)
+    (fun state =>
+       {| pre := logical_abstraction state ps ls;
+          post state' r :=
+            state' = state /\
+            index ls.(ls_disk) a ?|= eq r;
+          alternate state' r :=
+            exists ps' ls',
+              logical_abstraction state' ps' ls' /\
+              ls'.(ls_committed) = false /\
+              ls'.(ls_log) = nil /\
+              ls'.(ls_disk) = ls.(ls_disk);
+       |}).
+Proof.
+  eapply mk_rspec; eauto; simpl.
+  - intros.
+    destruct a0.
+    destruct x.
+    eapply recovery_ok.
+  - eapply log_apply_spec_idempotent_crash_step'.
+  - intros.
+    inv_clear H1.
+    eexists (exist _ (_, _) _).
+    simpl.
+    intuition eauto.
+  - unfold logical_abstraction; propositional.
+    destruct a0.
+    destruct x.
+    simpl in *; propositional.
+    descend.
+    repeat match goal with
+           | [ |- _ /\ _ ] => split
+           end; eauto.
+    Unshelve.
+    simpl; auto.
+Qed.
+
+Definition abstraction (txnd: TxnD.State) (d: D.State) (u: unit) : Prop :=
+  exists ps ls,
+    PhyDecode d ps /\
+    LogDecode ps ls /\
+    ls.(ls_committed) = false.
